removed InjectPerm from StackADT

common/StackADT.v
@@ -620,23 +620,12 @@ Proof.
   rewrite in_stack_cons; left. eauto.
 Qed.
 
-(** * Surjectivity of stack injections  *)
-
-(* Definition frameinj_surjective (g: frameinj) n2 := *)
-(*   sum_list g = n2. *)
-
-Class InjectPerm :=
-  {
-    inject_perm_condition: permission -> Prop;
-    inject_perm_condition_writable: forall p, perm_order Writable p -> inject_perm_condition p;
-  }.
-
 (** * Specifying tailcalled frames.  *)
 (** A tframe is a non-empty list of frames (a::l). It must be the case that all
     blocks in l have no permission.
  *)
 
-Definition wf_tframe (m: perm_type) (* (j: meminj) *) (tf: tframe_adt) : Prop :=
+Definition wf_tframe (m: perm_type) (tf: tframe_adt) : Prop :=
   forall b,
     forall f,
       In f (snd tf) ->
@@ -648,13 +637,11 @@ Definition wf_stack (m: perm_type) (s: stack) : Prop :=
   Forall (wf_tframe m) s.
 
 Section INJ.
-  Context {injperm: InjectPerm}.
-
    Definition has_perm (m: perm_type) (j: meminj) (f: tframe_adt) : Prop :=
-     exists b o k p, j b <> None /\ in_frames f b /\ m b o k p /\ inject_perm_condition p.
+     exists b o k p, j b <> None /\ in_frames f b /\ m b o k p.
 
    Definition has_perm_frame (m: perm_type) (j: meminj) (f: frame_adt) : Prop :=
-     exists b o k p, j b <> None /\ in_frame f b /\ m b o k p /\ inject_perm_condition p.
+     exists b o k p, j b <> None /\ in_frame f b /\ m b o k p.
 
    Definition tframe_inject (f: meminj) (P: perm_type) (tf1 tf2: tframe_adt): Prop :=
      forall f1,
@@ -687,7 +674,7 @@ Section INJ.
        tframe_inject f P f1 f2 ->
        tframe_inject f' P f1 f2.
    Proof.
-     intros P f f' f1 f2 INCR NEW TF ff1 IN1 (b & o & k & p & Fnone & IFR & PERM & IPC).
+     intros P f f' f1 f2 INCR NEW TF ff1 IN1 (b & o & k & p & Fnone & IFR & PERM).
      edestruct TF as (f0 & IN & FI); eauto.
      - red.
        repeat eexists; eauto.
@@ -708,12 +695,11 @@ Section INJ.
        (PERMS: forall b1 b2 delta o k p,
            f b1 = Some (b2, delta) ->
            P b1 o k p ->
-           inject_perm_condition p ->
            P' b2 (o + delta)%Z k p),
        tframe_inject (compose_meminj f f') P l1 l3.
    Proof.
      intros f f' P P' l1 l2 FI12 l3 FI23 PERMS
-            f1 INf1 (b & o & k & p & JB & IFR & PERM & IPC).
+            f1 INf1 (b & o & k & p & JB & IFR & PERM).
      unfold compose_meminj in JB; repeat destr_in JB. subst.
      edestruct FI12 as (f2 & INl2 & FI12'); eauto.
      repeat eexists; eauto. congruence.
@@ -800,7 +786,7 @@ Section INJ.
     forall b1 b2 delta bi1,
       f b1 = Some (b2, delta) ->
       in_stack' s1 (b1, bi1) ->
-      (exists o k p, P b1 o k p /\ inject_perm_condition p) ->
+      (exists o k p, P b1 o k p) ->
       exists bi2,
         in_stack' s2 (b2, bi2) /\ inject_frame_info delta bi1 bi2.
   Proof.
@@ -809,7 +795,7 @@ Section INJ.
     induction 1; simpl; intros b1 b2 delta bi1 FB INS PERM.
     - easy.
     - subst.
-      destruct PERM as (o & k & p & PERM & IPC).
+      destruct PERM as (o & k & p & PERM).
       rewrite (take_drop _ _ _ TAKE) in INS.
       rewrite in_stack'_app in INS.
       destruct INS as [INS|INS].
@@ -855,9 +841,9 @@ Section INJ.
 
   Lemma tframe_inject_in_frames:
     forall f m v1 v2 b b' delta o k p,
-      tframe_inject f m v1 v2 -> m b o k p -> inject_perm_condition p -> in_frames v1 b -> f b = Some (b', delta) -> in_frames v2 b'.
+      tframe_inject f m v1 v2 -> m b o k p -> in_frames v1 b -> f b = Some (b', delta) -> in_frames v2 b'.
   Proof.
-    intros f m v1 v2 b b' delta o k p TFI PERM IPC IFR FB.
+    intros f m v1 v2 b b' delta o k p TFI PERM IFR FB.
     red in IFR. unfold get_opt_frame_blocks in IFR.
     destr_in IFR; try easy. unfold get_frame_blocks in IFR.
     rewrite in_map_iff in IFR. destruct IFR as (fa & blocks & IN). subst.
@@ -876,7 +862,7 @@ Section INJ.
       stack_inject f m g s1 s2 ->
       forall b1 b2 delta,
         f b1 = Some (b2, delta) ->
-        (exists o k p, m b1 o k p /\ inject_perm_condition p) ->
+        (exists o k p, m b1 o k p) ->
         is_stack_top s1 b1 ->
         is_stack_top s2 b2.
   Proof.
@@ -888,7 +874,7 @@ Section INJ.
     constructor. reflexivity.
     inv FAP1. inv H.
     simpl in TAKE. destr_in TAKE. inv TAKE. inv FI.
-    destruct PERM as (o & k & p & PERM & IPC).
+    destruct PERM as (o & k & p & PERM).
     eapply tframe_inject_in_frames; eauto.
   Qed.
 
@@ -1153,12 +1139,11 @@ Section INJ.
           f b1 = Some (b2, delta) ->
           forall o k p,
             m b1 o k p ->
-            inject_perm_condition p ->
         inject_frame_info delta bi1 bi2.
   Proof.
     intros f g m l1 l2 SI ND1 ND2 b1 bi1 b2 bi2 INS1 INS2 delta FB o k p PERM IPC.
     edestruct (stack_inject_compat _ _ _ _ _ SI _ _ _ _ FB INS1) as (bi2' & INS2' & IFI).
-    do 3 eexists; split; eauto.
+    do 3 eexists; eauto.
     cut (bi2 = bi2'). intro; subst; auto.
     eapply in_stack'_norepet; eauto.
   Qed.
@@ -1269,7 +1254,6 @@ Section INJ.
       (PERMS: forall b1 b2 delta o k p,
           f b1 = Some (b2, delta) ->
           m1 b1 o k p ->
-          inject_perm_condition p ->
           m2 b2 (o + delta)%Z k p),
       stack_inject (compose_meminj f f') m1 g3 s1 s3.
   Proof.
@@ -1307,7 +1291,6 @@ Section INJ.
         (forall b1 b2 delta o k p,
             f b1 = Some (b2, delta) ->
             m1 b1 o k p ->
-            inject_perm_condition p ->
             m2 b2 (o + delta)%Z k p) ->
         stack_agree_perms m2 l2 ->
         forall g3,
@@ -1439,7 +1422,7 @@ Section INJ.
       (ND1: nodup s1)
       (ND2: nodup s2)
       (FB : f b1 = Some (b2, delta))
-      (PERM: exists o k p, m1 b1 o k p /\ inject_perm_condition p),
+      (PERM: exists o k p, m1 b1 o k p),
       option_le_stack (fun fi => True) (* this correct? *)
                 (inject_frame_info delta)
                 delta
@@ -1451,7 +1434,7 @@ Section INJ.
     destruct (in_stack_dec s1 b1).
     edestruct in_stack_in_frames_ex as (ff & INS & INF); eauto.
     destruct (get_assoc_stack s1 b1) eqn:STK1.
-    - destruct PERM as (o & k & p & PERM & IPC).
+    - destruct PERM as (o & k & p & PERM).
       eapply (wf_stack_in_frames_in_frame) in INF; eauto.
       destruct INF as (vf1 & VF1 & INF).
       edestruct in_frame_info as (fi2 & INF2); eauto.
@@ -1477,7 +1460,7 @@ Section INJ.
     forall P f g s1 s2 b1 b2 delta
       (MINJ: stack_inject f P g s1 s2)
       (FB: f b1 = Some (b2, delta))
-      (PERM: exists o k p, P b1 o k p /\ inject_perm_condition p)
+      (PERM: exists o k p, P b1 o k p)
       (IST: is_stack_top s1 b1),
       is_stack_top s2 b2.
   Proof.
@@ -1531,7 +1514,7 @@ Lemma tframe_inject_invariant:
 Proof.
   intros m m' f f1 f2 thr PERMS PLT TFI ff1 INf1 HP.
   specialize (TFI _ INf1).
-  trim TFI. destruct HP as (b & o & k & p & FB & IFR & PERM & IPC).
+  trim TFI. destruct HP as (b & o & k & p & FB & IFR & PERM).
   destruct (f b) eqn:?; try congruence. destruct p0.
   repeat eexists; eauto. congruence. eapply PERMS; eauto.
   eapply PLT; eauto. eapply in_frame_in_frames; eauto.
@@ -1548,7 +1531,7 @@ Lemma tframe_inject_invariant_strong:
     tframe_inject f m' f1 f2.
 Proof.
   intros m m' f f1 f2 PERMS TFI ff1 INf1 HP.
-  specialize (TFI _ INf1). trim TFI. destruct HP as (b & o & k & p & FB & IFR & PERM & IPC).
+  specialize (TFI _ INf1). trim TFI. destruct HP as (b & o & k & p & FB & IFR & PERM).
   destruct (f b) eqn:?; try congruence. destruct p0.
   repeat eexists; eauto. congruence.
   destruct TFI as (f3 & EQ & FI).
@@ -1626,7 +1609,7 @@ Lemma tframe_inject_invariant':
 Proof.
   intros m m' f f1 f2 PERMS TFI ff1 INf1 HP.
   specialize (TFI _ INf1).
-  trim TFI. destruct HP as (b & o & k & p & FB & IFR & PERM & IPC).
+  trim TFI. destruct HP as (b & o & k & p & FB & IFR & PERM).
   destruct (f b) eqn:?; try congruence. destruct p0.
   repeat eexists; eauto. congruence. eapply PERMS; eauto.
   left. rewrite INf1. simpl. auto.
@@ -2091,7 +2074,7 @@ Lemma has_perm_frame_ext:
     has_perm_frame P j f ->
     has_perm_frame P j' f.
 Proof.
-  intros j j' P f EXT (b & o & k & p0 & FSOME & INFR1 & PERM & IPC).
+  intros j j' P f EXT (b & o & k & p0 & FSOME & INFR1 & PERM).
   repeat eexists; eauto. rewrite EXT in FSOME; auto.
 Qed.
 
@@ -2365,24 +2348,14 @@ Proof.
 Qed.
 End INJ.
 
-Program Definition inject_perm_upto_writable: InjectPerm :=
-  {|
-    inject_perm_condition := fun p => perm_order Writable p
-  |}.
-
-Program Definition inject_perm_all: InjectPerm :=
-  {|
-    inject_perm_condition := fun p => True
-  |}.
-
-Lemma has_perm_frame_impl {injperm: InjectPerm}:
+Lemma has_perm_frame_impl:
   forall (P1 P2: perm_type) j f tf,
     has_perm_frame P1 j f ->
     frame_inject j f tf ->
-    (forall b1 b2 delta o k p, j b1 = Some (b2, delta) -> P1 b1 o k p -> inject_perm_condition p -> P2 b2 (o + delta)%Z k p) ->
+    (forall b1 b2 delta o k p, j b1 = Some (b2, delta) -> P1 b1 o k p -> P2 b2 (o + delta)%Z k p) ->
     has_perm_frame P2 inject_id tf.
 Proof.
-  intros P1 P2 j f tf (b & o & k & p & NONE & IFR & PERM1 & IPC) FI PERMS.
+  intros P1 P2 j f tf (b & o & k & p & NONE & IFR & PERM1) FI PERMS.
   red in FI.
   apply in_frame_info in IFR. destruct IFR as (fi & IFR).
   rewrite Forall_forall in FI; specialize (FI _ IFR).
@@ -2391,7 +2364,7 @@ Proof.
   specialize (FI _ _ eq_refl).
   destruct FI as (fi' & IN' & IFI).
   exists b0, (o + z)%Z, k, p. split. unfold inject_id. congruence.
-  split. eapply in_frame'_in_frame; eauto. split; eauto.
+  split. eapply in_frame'_in_frame; eauto. eauto.
 Qed.
 
 Definition stack_top_is_new s :=
